

União a tripla de Hesse:

$$\vdash \langle x > 0 \rangle \text{ Prova } \langle ((x = 2y) \wedge (z = -1)) \vee ((x = 2y + 1) \wedge (z = 3x)) \rangle$$

teremos a tabela:

Regra:	para	Aserção:	Programa:
/		/	/
		p. : Verificado e Correto!	
Implicação	5	$x > 0 \wedge \text{mod}(x, 2) = 0 \rightarrow ((x = 2y) \wedge (-1 = -1)) \vee ((x = 2y + 1) \wedge (-1 = 3x))$ $\wedge (\neg \text{mod}(x, 2) = 0 \rightarrow ((x = 2y) \wedge (3x = -1)) \vee ((x = 2y + 1) \wedge (3x = 3x)))$	
Atribuição	4	$(\text{mod}(x, 2) = 0 \rightarrow ((x = 2y) \wedge (-1 = -1)) \vee ((x = 2y + 1) \wedge (-1 = 3x)))$ $\wedge (\neg \text{mod}(x, 2) = 0 \rightarrow ((x = 2y) \wedge (3x = -1)) \vee ((x = 2y + 1) \wedge (3x = 3x)))$	$a := 3x;$
If-Else	3	$(\text{mod}(x, 2) = 0 \rightarrow ((x = 2y) \wedge (-1 = -1)) \vee ((x = 2y + 1) \wedge (-1 = 3x)))$ $\wedge (\neg \text{mod}(x, 2) = 0 \rightarrow ((x = 2y) \wedge (a = -1)) \vee ((x = 2y + 1) \wedge (a = 3x)))$	$\text{if } (\text{mod}(x, 2) = 0) \{$
Atribuição	2	$((x = 2y) \wedge (-1 = -1)) \vee ((x = 2y + 1) \wedge (-1 = 3x))$	$z := -1;$
If-Else	1	$((x = 2y) \wedge (z = -1)) \vee ((x = 2y + 1) \wedge (z = 3x))$	$\{$
			$\text{else } \{$
Atribuição	2	$((x = 2y) \wedge (a = -1)) \vee ((x = 2y + 1) \wedge (a = 3x))$	$z := a;$
If-Else	1	$((x = 2y) \wedge (z = -1)) \vee ((x = 2y + 1) \wedge (z = 3x))$	$\}$
	0	$((x = 2y) \wedge (z = -1)) \vee ((x = 2y + 1) \wedge (z = 3x))$	